compiler/backend/proofs/clos_callProofScript.sml
@@ -336,7 +336,6 @@ val wfv_ind = theorem"wfv_ind";
 val wfv_state_def = Define`
   wfv_state g l code s ⇔
     EVERY (OPTION_ALL (wfv g l code)) s.globals ∧
-    (OPTION_ALL (wfv g l code)) s.mutable_global ∧
     FEVERY (every_refv (wfv g l code) o SND) s.refs ∧
     s.code = FEMPTY`;
 
@@ -349,7 +348,6 @@ val state_rel_def = Define`
     (s.clock = t.clock) ∧
     (s.max_app = t.max_app) ∧
     LIST_REL (OPTREL (v_rel g l t.code)) s.globals t.globals ∧
-    (OPTREL (v_rel g l t.code)) s.mutable_global t.mutable_global /\
     fmap_rel (ref_rel (v_rel g l t.code)) s.refs t.refs ∧
     s.code = FEMPTY`;
 
@@ -1929,8 +1927,6 @@ Proof
       \\ qspec_tac (`s2.globals`,`w`) \\ Induct \\ fs []
       \\ Cases \\ fs [OPTREL_def])
     THEN1
-      (Cases_on`s2.mutable_global`>>fs[OPTREL_def])
-    THEN1
       (match_mp_tac (FEVERY_STRENGTHEN_THM |> CONJUNCT2) \\ fs [])
     THEN1
       (match_mp_tac (FEVERY_STRENGTHEN_THM |> CONJUNCT2) \\ fs []
@@ -1952,10 +1948,7 @@ Proof
       (qsuff_tac `xs = ys` \\ fs []
        \\ qpat_x_assum `_ xs ys` mp_tac
        \\ qspec_tac (`xs`,`xs`) \\ qspec_tac (`ys`,`ys`)
-       \\ Induct \\ fs [PULL_EXISTS] \\ Cases  \\ Cases \\ fs [OPTREL_def])
-    THEN1 (Cases_on`x`>> fs[OPTREL_def])
-    THEN1 (Cases_on`x`>> fs[OPTREL_def])
-    )
+       \\ Induct \\ fs [PULL_EXISTS] \\ Cases  \\ Cases \\ fs [OPTREL_def]))
   \\ fs [AC CONJ_ASSOC CONJ_COMM]
   \\ rpt (disch_then assume_tac) \\ fs [AND_IMP_INTRO]
   \\ first_x_assum match_mp_tac
@@ -2198,13 +2191,6 @@ Proof
   \\ conj_tac >- (
     first_x_assum (fn t => mp_tac t \\ match_mp_tac LIST_REL_mono)
     \\ rpt gen_tac
-    \\ match_mp_tac OPTREL_MONO
-    \\ rw []
-    \\ drule_then irule (GEN_ALL v_rel_SUBMAP_subg)
-    \\ fs [SUBMAP_FUNION_ID, DISJOINT_SYM]
-  )
-  \\ conj_tac >- (
-    qpat_x_assum `OPTREL _ _ _` mp_tac
     \\ match_mp_tac OPTREL_MONO
     \\ rw []
     \\ drule_then irule (GEN_ALL v_rel_SUBMAP_subg)
